add outcome in mlanguage

theories/mlanguage/mlanguage.v
@@ -6,8 +6,8 @@ From melocoton Require Export multirelations language_commons.
 Section mlanguage_mixin.
   Context {expr val func state ectx : Type}.
 
-  Context (of_val : val → expr).
-  Context (to_val : expr → option val).
+  Context (of_outcome : outcome val → expr).
+  Context (to_outcome : expr → option (outcome val)).
 
   Context (to_call : string → list val → expr).
   Context (is_call : expr → string → list val → ectx → Prop).
@@ -23,21 +23,21 @@ Section mlanguage_mixin.
   Context (prim_step : mixin_prog → umrel (expr * state)).
 
   Record MlanguageMixin := {
-    (** Expression and values *)
-    mixin_to_of_val c : to_val (of_val c) = Some c;
-    mixin_of_to_val e c : to_val e = Some c → of_val c = e;
+    (** Expression and outcomes *)
+    mixin_to_of_outcome o : to_outcome (of_outcome o) = Some o;
+    mixin_of_to_outcome e o : to_outcome e = Some o → of_outcome o = e;
 
     (** Reduction behavior of the special classes of expressions *)
-    (** mixin_val_prim_step is not an iff because the backward direction is trivial *)
-    mixin_val_prim_step p v σ :
-      prim_step p (of_val v, σ) (λ _, False);
+    (** mixin_outcome_prim_step is not an iff because the backward direction is trivial *)
+    mixin_outcome_prim_step p v σ :
+      prim_step p (of_outcome v, σ) (λ _, False);
     mixin_call_prim_step p e f vs K σ X :
       is_call e f vs K →
         prim_step p (e, σ) X ↔
         (∃ (fn : func) (e2 : expr),
           p !! f = Some fn ∧ Some e2 = apply_func fn vs ∧ X (fill K e2, σ));
 
-    mixin_is_val_not_call e : is_Some (to_val e) → (∀ f vs K, ¬ is_call e f vs K);
+    mixin_is_outcome_not_call e : is_Some (to_outcome e) → (∀ f vs K, ¬ is_call e f vs K);
     mixin_is_call_in_ctx e K1 K2 s vv :
       is_call e s vv K2 → is_call (fill K1 e) s vv (comp_ectx K1 K2);
     mixin_to_call_is_call fn vs : is_call (to_call fn vs) fn vs empty_ectx;
@@ -46,14 +46,16 @@ Section mlanguage_mixin.
       is_call (to_call fn vs) fn' vs' K →
       fn' = fn ∧ vs' = vs ∧ K = empty_ectx;
 
-    mixin_resume_val e K : is_Some (to_val (fill K e)) → is_Some (to_val e);
+    mixin_resume_outcome e K :
+      is_Some (to_outcome (fill K e)) →
+      to_outcome (fill K e) = to_outcome e;
     mixin_resume_compose e K1 K2 :
       fill K1 (fill K2 e) = fill (comp_ectx K1 K2) e;
     mixin_resume_empty e :
       fill empty_ectx e = e;
 
     mixin_prim_step_resume p K e σ X :
-      to_val e = None →
+      to_outcome e = None →
       prim_step p (e, σ) X →
       prim_step p (fill K e, σ) (λ '(e2, σ2),
         ∃ e', e2 = fill K e' ∧ X (e', σ2));
@@ -61,13 +63,12 @@ Section mlanguage_mixin.
     (* Just a meta-theorem to ensure that there are no cases left to cover.
        Not used in proofs. *)
     mixin_prim_step_no_NB p e σ X :
-      to_val e = None →
+      to_outcome e = None →
       prim_step p (e, σ) X →
       ∃ e' σ', X (e', σ');
   }.
 End mlanguage_mixin.
 
-Arguments mixin_expr_class : clear implicits.
 Global Notation mixin_prog func := (gmap string func).
 
 Structure mlanguage {val : Type} := Mlanguage {
@@ -76,8 +77,8 @@ Structure mlanguage {val : Type} := Mlanguage {
   state : Type;
   ectx : Type;
 
-  of_val : val → expr;
-  to_val : expr → option val;
+  of_outcome : outcome val → expr;
+  to_outcome : expr → option (outcome val);
 
   to_call : string → list val → expr;
   is_call : expr → string → list val → ectx → Prop;
@@ -90,7 +91,7 @@ Structure mlanguage {val : Type} := Mlanguage {
 
 
   mlanguage_mixin :
-    MlanguageMixin (val:=val) of_val to_val to_call is_call empty_ectx
+    MlanguageMixin (val:=val) of_outcome to_outcome to_call is_call empty_ectx
       comp_ectx fill apply_func prim_step
 }.
 
@@ -99,8 +100,8 @@ Bind Scope expr_scope with expr.
 
 Arguments mlanguage : clear implicits.
 Arguments Mlanguage {_ expr _ _ _ _ _ _ _ _ _ fill apply_func prim_step}.
-Arguments of_val {_} _ _.
-Arguments to_val {_ _} _.
+Arguments of_outcome {_} _ _.
+Arguments to_outcome {_ _} _.
 Arguments to_call {_} _ _.
 Arguments is_call {_ _}.
 Arguments empty_ectx {_ _}.
@@ -121,18 +122,46 @@ Section mlanguage.
   Implicit Types p : prog Λ.
   Implicit Types X : expr Λ * state Λ → Prop.
 
-  Lemma to_of_val c : to_val (of_val Λ c) = Some c.
+  Lemma to_of_outcome o : to_outcome (of_outcome Λ o) = Some o.
   Proof. apply mlanguage_mixin. Qed.
-  Lemma of_to_val e c : to_val e = Some c → of_val Λ c = e.
+  Lemma of_to_outcome e o : to_outcome e = Some o → of_outcome Λ o = e.
   Proof. apply mlanguage_mixin. Qed.
+
+  Definition of_val Λ v := of_outcome Λ (OVal v).
+  Definition to_val e : option val :=
+    match to_outcome e with
+    | Some (OVal v) => Some v
+    | _ => None
+    end.
+
+  Lemma of_outcome_of_val v : of_outcome Λ (OVal v) = of_val Λ v.
+  Proof. easy. Qed.
+  Lemma to_outcome_of_val v : to_outcome (of_val Λ v) = Some (OVal v).
+  Proof. rewrite /of_val to_of_outcome //. Qed.
+
+  Lemma to_of_val v : to_val (of_val Λ v) = Some v.
+  Proof. rewrite /to_val to_of_outcome //. Qed.
+  Lemma of_to_val e v : to_val e = Some v → of_val Λ v = e.
+  Proof.
+    unfold to_val, of_val.
+    destruct (to_outcome e) eqn:Heq; try destruct o; try congruence.
+    inversion 1; subst. now apply of_to_outcome in Heq. 
+  Qed.
+
+  Lemma of_outcome_inj k1 k2 : of_outcome Λ k1 = of_outcome Λ k2 → k1 = k2.
+  Proof.
+    intros H. enough (Some k1 = Some k2) by congruence.
+    rewrite <- !to_of_outcome. rewrite H. done.
+  Qed.
 
   Lemma of_val_inj k1 k2 : of_val Λ k1 = of_val Λ k2 → k1 = k2.
   Proof.
     intros H. enough (Some k1 = Some k2) by congruence.
     rewrite <- !to_of_val. rewrite H. done.
   Qed.
-  Lemma val_prim_step p v σ :
-    prim_step p (of_val Λ v, σ) (λ _, False).
+
+  Lemma outcome_prim_step p o σ :
+    prim_step p (of_outcome Λ o, σ) (λ _, False).
   Proof. apply mlanguage_mixin. Qed.
   Lemma call_prim_step p e f vs K σ X :
       is_call e f vs K →
@@ -144,14 +173,14 @@ Section mlanguage.
   Definition not_is_call e : Prop := ¬ ∃ f vs K, is_call e f vs K.
   Definition not_is_ext_call (p : prog Λ) e : Prop := ¬ ∃ f vs K, is_call e f vs K ∧ p !! f = None.
 
-  Lemma is_val_not_call e : is_Some (to_val e) → (∀ f vs K, ¬ is_call e f vs K).
+  Lemma is_outcome_not_call e : is_Some (to_outcome e) → (∀ f vs K, ¬ is_call e f vs K).
   Proof. apply mlanguage_mixin. Qed.
 
-  Lemma is_val_not_call_2 e f vs K : is_call e f vs K → to_val e = None.
+  Lemma is_outcome_not_call_2 e f vs K : is_call e f vs K → to_outcome e = None.
   Proof.
-    intros H; destruct (to_val e) eqn:Heq; try done.
+    intros H; destruct (to_outcome e) eqn:Heq; try done.
     exfalso; apply mk_is_Some in Heq.
-    eapply is_val_not_call in Heq. done.
+    eapply is_outcome_not_call in Heq. done.
   Qed.
 
   Lemma is_call_in_ctx e K1 K2 s vv :
@@ -167,13 +196,20 @@ Section mlanguage.
     fn' = fn ∧ vs' = vs ∧ K = empty_ectx.
   Proof. apply mlanguage_mixin. Qed.
 
-  Lemma resume_val e K : is_Some (to_val (fill K e)) → is_Some (to_val e).
+  Lemma resume_outcome e K :
+    is_Some (to_outcome (fill K e)) → to_outcome (fill K e) = to_outcome e.
   Proof. apply mlanguage_mixin. Qed.
 
-  Lemma resume_not_val e K : to_val e = None → to_val (fill K e) = None.
+  Lemma resume_outcome_2 e K : is_Some (to_outcome (fill K e)) → is_Some (to_outcome e).
   Proof.
-    intros Heq; destruct (to_val (fill K e)) as [v|] eqn:Heq2; last done.
-    eapply mk_is_Some in Heq2. apply resume_val in Heq2. rewrite Heq in Heq2.
+    intros H. assert (is_Some (to_outcome (fill K e))) as [x Heq] by done.
+    apply resume_outcome in H. rewrite Heq in H; done.
+  Qed.
+
+  Lemma resume_not_outcome e K : to_outcome e = None → to_outcome (fill K e) = None.
+  Proof.
+    intros Heq; destruct (to_outcome (fill K e)) as [v|] eqn:Heq2; last done.
+    eapply mk_is_Some in Heq2. apply resume_outcome_2 in Heq2; rewrite Heq in Heq2.
     by destruct Heq2.
   Qed.
 
@@ -185,13 +221,13 @@ Section mlanguage.
   Proof. apply mlanguage_mixin. Qed.
 
   Lemma prim_step_resume p K e σ X :
-    to_val e = None →
+    to_outcome e = None →
     prim_step p (e, σ) X →
     prim_step p (fill K e, σ) (λ '(e2, σ2), ∃ e', e2 = fill K e' ∧ X (e', σ2)).
   Proof. apply mlanguage_mixin. Qed.
 
   (* There is no NB *)
-  Lemma prim_step_no_NB p e σ X : to_val e = None → prim_step p (e,σ) X → ∃ e' σ', X (e', σ').
+  Lemma prim_step_no_NB p e σ X : to_outcome e = None → prim_step p (e,σ) X → ∃ e' σ', X (e', σ').
   Proof. apply mlanguage_mixin. Qed.
 
   Class IntoVal (e : expr Λ) (v : val) :=
@@ -207,8 +243,8 @@ Section mlanguage.
   Qed.
 
   (* Non-values must step to a set. By prim_step_no_NB, this set is not empty. *)
-  Definition safe p (e : expr Λ) (σ : state Λ) (Φ : val → Prop) := match to_val e with
-    Some v => Φ v
+  Definition safe p (e : expr Λ) (σ : state Λ) (Φ : outcome val → Prop) := match to_outcome e with
+    Some o => Φ o
   | None => ∃ X, prim_step p (e,σ) X end.
 
 End mlanguage.
